src/kem/kyber/hash_functions.rs
@@ -1,11 +1,10 @@
 #![allow(non_snake_case)]
 
-use crate::digest::{
-    self, digest_size, shake128_free, shake128_init_absorb, shake128_squeeze_nblocks, Algorithm,
-    Shake128State,
-};
-
 use super::constants::H_DIGEST_SIZE;
+use crate::{
+    digest::{self, digest_size, Algorithm},
+    sha3,
+};
 
 pub(crate) fn G(input: &[u8]) -> [u8; digest_size(Algorithm::Sha3_512)] {
     digest::sha3_512(input)
@@ -19,28 +18,74 @@ pub(crate) fn PRF<const LEN: usize>(input: &[u8]) -> [u8; LEN] {
     digest::shake256::<LEN>(input)
 }
 
-#[inline(always)]
-pub(crate) fn XOF_absorb<const K: usize>(input: [[u8; 34]; K]) -> [Shake128State; K] {
-    shake128_init_absorb(input)
+pub(crate) struct Shake128State<const K: usize> {
+    #[cfg(not(simd256))]
+    state: [sha3::incremental::Shake128State; K],
+    #[cfg(simd256)]
+    state: [sha3::incremental_x4::Shake128State; K],
+}
+
+impl<const K: usize> Shake128State<K> {
+    fn new() -> Self {
+        #[cfg(simd256)]
+        if simd256_support() {
+            Self {
+                state: core::array::from_fn(|_| sha3::incremental_x4::Shake128State::new()),
+            }
+        } else {
+            Self {
+                state: core::array::from_fn(|_| sha3::incremental::Shake128State::new()),
+            }
+        }
+        #[cfg(not(simd256))]
+        Self {
+            state: core::array::from_fn(|_| sha3::incremental::Shake128State::new()),
+        }
+    }
 }
 
 #[inline(always)]
-pub(crate) fn XOF_squeeze_three_blocks<const K: usize>(
-    mut xof_state: [Shake128State; K],
-) -> ([[u8; 168 * 3]; K], [Shake128State; K]) {
-    let output = shake128_squeeze_nblocks(&mut xof_state);
-    (output, xof_state)
+pub(crate) fn absorb<const K: usize>(input: [[u8; 34]; K]) -> Shake128State<K> {
+    debug_assert!(K == 2 || K == 3 || K == 4);
+
+    let mut states = Shake128State::new();
+    for i in 0..K {
+        states.state[i].absorb_final(&input[i]);
+    }
+    states
+}
+
+const BLOCK_SIZE: usize = 168;
+const THREE_BLOCKS: usize = BLOCK_SIZE * 3;
+
+#[inline(always)]
+pub(crate) fn squeeze_three_blocks<const K: usize>(
+    xof_state: &mut Shake128State<K>,
+) -> [[u8; THREE_BLOCKS]; K] {
+    let mut out = [[0u8; THREE_BLOCKS]; K];
+    for i in 0..K {
+        out[i] = xof_state.state[i].squeeze_nblocks();
+    }
+    out
 }
 
 #[inline(always)]
-pub(crate) fn XOF_squeeze_block<const K: usize>(
-    mut xof_state: [Shake128State; K],
-) -> ([[u8; 168]; K], [Shake128State; K]) {
-    let output = shake128_squeeze_nblocks(&mut xof_state);
-    (output, xof_state)
+pub(crate) fn squeeze_block<const K: usize>(
+    xof_state: &mut Shake128State<K>,
+) -> [[u8; BLOCK_SIZE]; K] {
+    let mut out = [[0u8; BLOCK_SIZE]; K];
+    for i in 0..K {
+        out[i] = xof_state.state[i].squeeze_nblocks();
+    }
+    out
 }
 
+/// Free the memory of the state.
+///
+/// **NOTE:** That this needs to be done manually for now.
 #[inline(always)]
-pub(crate) fn XOF_free<const K: usize>(xof_state: [Shake128State; K]) {
-    shake128_free(xof_state);
+pub(crate) fn free<const K: usize>(mut xof_state: Shake128State<K>) {
+    for i in 0..K {
+        xof_state.state[i].free();
+    }
 }
