proofs/fstar/extraction/Libcrux.Kem.Kyber.Hash_functions.fst
@@ -9,35 +9,174 @@ let v_H (input: t_Slice u8) = Libcrux.Digest.sha3_256_ input
 
 let v_PRF (v_LEN: usize) (input: t_Slice u8) = Libcrux.Digest.shake256 v_LEN input
 
-let v_XOF_absorb (v_K: usize) (input: t_Array (t_Array u8 (sz 34)) v_K) =
-  let state:t_Array Libcrux.Digest.t_Shake128State v_K =
-    Libcrux.Digest.impl__Shake128State__new v_K ()
-  in
-  let state:t_Array Libcrux.Digest.t_Shake128State v_K =
-    Libcrux.Digest.shake128_absorb_final v_K state input
-  in
-  state
-
-let v_XOF_free (v_K: usize) (xof_state: t_Array Libcrux.Digest.t_Shake128State v_K) =
-  let _:Prims.unit = Libcrux.Digest.shake128_free v_K xof_state in
-  ()
-
-let v_XOF_squeeze_block (v_K: usize) (xof_state: t_Array Libcrux.Digest.t_Shake128State v_K) =
-  let tmp0, out:(t_Array Libcrux.Digest.t_Shake128State v_K & t_Array (t_Array u8 (sz 168)) v_K) =
-    Libcrux.Digest.shake128_squeeze_nblocks (sz 168) v_K xof_state
-  in
-  let xof_state:t_Array Libcrux.Digest.t_Shake128State v_K = tmp0 in
-  let output:t_Array (t_Array u8 (sz 168)) v_K = out in
-  output, xof_state
+let impl__new (v_K: usize) (_: Prims.unit) =
+  {
+    f_state
+    =
+    Core.Array.from_fn v_K
+      (fun temp_0_ ->
+          let _:usize = temp_0_ in
+          Libcrux.Hacl.Sha3.Incremental.impl__Shake128State__new ()
+          <:
+          Libcrux.Hacl.Sha3.Incremental.t_Shake128State)
+  }
   <:
-  (t_Array (t_Array u8 (sz 168)) v_K & t_Array Libcrux.Digest.t_Shake128State v_K)
+  t_Shake128State v_K
 
-let v_XOF_squeeze_three_blocks (v_K: usize) (xof_state: t_Array Libcrux.Digest.t_Shake128State v_K) =
-  let tmp0, out:(t_Array Libcrux.Digest.t_Shake128State v_K & t_Array (t_Array u8 (sz 504)) v_K) =
-    Libcrux.Digest.shake128_squeeze_nblocks (sz 504) v_K xof_state
+let absorb (v_K: usize) (input: t_Array (t_Array u8 (sz 34)) v_K) =
+  let _:Prims.unit =
+    if true
+    then
+      let _:Prims.unit =
+        if ~.((v_K =. sz 2 <: bool) || (v_K =. sz 3 <: bool) || (v_K =. sz 4 <: bool))
+        then
+          Rust_primitives.Hax.never_to_any (Core.Panicking.panic "assertion failed: K == 2 || K == 3 || K == 4"
+
+              <:
+              Rust_primitives.Hax.t_Never)
+      in
+      ()
   in
-  let xof_state:t_Array Libcrux.Digest.t_Shake128State v_K = tmp0 in
-  let output:t_Array (t_Array u8 (sz 504)) v_K = out in
-  output, xof_state
-  <:
-  (t_Array (t_Array u8 (sz 504)) v_K & t_Array Libcrux.Digest.t_Shake128State v_K)
+  let states:t_Shake128State v_K = impl__new v_K () in
+  let states:t_Shake128State v_K =
+    Core.Iter.Traits.Iterator.f_fold (Core.Iter.Traits.Collect.f_into_iter ({
+              Core.Ops.Range.f_start = sz 0;
+              Core.Ops.Range.f_end = v_K
+            }
+            <:
+            Core.Ops.Range.t_Range usize)
+        <:
+        Core.Ops.Range.t_Range usize)
+      states
+      (fun states i ->
+          let states:t_Shake128State v_K = states in
+          let i:usize = i in
+          {
+            states with
+            f_state
+            =
+            Rust_primitives.Hax.Monomorphized_update_at.update_at_usize states.f_state
+              i
+              (Libcrux.Hacl.Sha3.Incremental.impl__Shake128State__absorb_final (states.f_state.[ i ]
+                    <:
+                    Libcrux.Hacl.Sha3.Incremental.t_Shake128State)
+                  (Rust_primitives.unsize (input.[ i ] <: t_Array u8 (sz 34)) <: t_Slice u8)
+                <:
+                Libcrux.Hacl.Sha3.Incremental.t_Shake128State)
+            <:
+            t_Array Libcrux.Hacl.Sha3.Incremental.t_Shake128State v_K
+          }
+          <:
+          t_Shake128State v_K)
+  in
+  states
+
+let free (v_K: usize) (xof_state: t_Shake128State v_K) =
+  Core.Iter.Traits.Iterator.f_fold (Core.Iter.Traits.Collect.f_into_iter ({
+            Core.Ops.Range.f_start = sz 0;
+            Core.Ops.Range.f_end = v_K
+          }
+          <:
+          Core.Ops.Range.t_Range usize)
+      <:
+      Core.Ops.Range.t_Range usize)
+    xof_state
+    (fun xof_state i ->
+        let xof_state:t_Shake128State v_K = xof_state in
+        let i:usize = i in
+        {
+          xof_state with
+          f_state
+          =
+          Rust_primitives.Hax.Monomorphized_update_at.update_at_usize xof_state.f_state
+            i
+            (Libcrux.Hacl.Sha3.Incremental.impl__Shake128State__free (xof_state.f_state.[ i ]
+                  <:
+                  Libcrux.Hacl.Sha3.Incremental.t_Shake128State)
+              <:
+              Libcrux.Hacl.Sha3.Incremental.t_Shake128State)
+          <:
+          t_Array Libcrux.Hacl.Sha3.Incremental.t_Shake128State v_K
+        }
+        <:
+        t_Shake128State v_K)
+
+let squeeze_block (v_K: usize) (xof_state: t_Shake128State v_K) =
+  let out:t_Array (t_Array u8 (sz 168)) v_K =
+    Rust_primitives.Hax.repeat (Rust_primitives.Hax.repeat 0uy (sz 168) <: t_Array u8 (sz 168)) v_K
+  in
+  let out, xof_state:(t_Array (t_Array u8 (sz 168)) v_K & t_Shake128State v_K) =
+    Core.Iter.Traits.Iterator.f_fold (Core.Iter.Traits.Collect.f_into_iter ({
+              Core.Ops.Range.f_start = sz 0;
+              Core.Ops.Range.f_end = v_K
+            }
+            <:
+            Core.Ops.Range.t_Range usize)
+        <:
+        Core.Ops.Range.t_Range usize)
+      (out, xof_state <: (t_Array (t_Array u8 (sz 168)) v_K & t_Shake128State v_K))
+      (fun temp_0_ i ->
+          let out, xof_state:(t_Array (t_Array u8 (sz 168)) v_K & t_Shake128State v_K) = temp_0_ in
+          let i:usize = i in
+          let tmp0, out1:(Libcrux.Hacl.Sha3.Incremental.t_Shake128State & t_Array u8 (sz 168)) =
+            Libcrux.Hacl.Sha3.Incremental.impl__Shake128State__squeeze_nblocks (sz 168)
+              (xof_state.f_state.[ i ] <: Libcrux.Hacl.Sha3.Incremental.t_Shake128State)
+          in
+          let xof_state:t_Shake128State v_K =
+            {
+              xof_state with
+              f_state
+              =
+              Rust_primitives.Hax.Monomorphized_update_at.update_at_usize xof_state.f_state i tmp0
+            }
+            <:
+            t_Shake128State v_K
+          in
+          let hoist1:t_Array u8 (sz 168) = out1 in
+          let hoist2:t_Array (t_Array u8 (sz 168)) v_K =
+            Rust_primitives.Hax.Monomorphized_update_at.update_at_usize out i hoist1
+          in
+          hoist2, xof_state <: (t_Array (t_Array u8 (sz 168)) v_K & t_Shake128State v_K))
+  in
+  let hax_temp_output:t_Array (t_Array u8 (sz 168)) v_K = out in
+  xof_state, hax_temp_output <: (t_Shake128State v_K & t_Array (t_Array u8 (sz 168)) v_K)
+
+let squeeze_three_blocks (v_K: usize) (xof_state: t_Shake128State v_K) =
+  let out:t_Array (t_Array u8 (sz 504)) v_K =
+    Rust_primitives.Hax.repeat (Rust_primitives.Hax.repeat 0uy (sz 504) <: t_Array u8 (sz 504)) v_K
+  in
+  let out, xof_state:(t_Array (t_Array u8 (sz 504)) v_K & t_Shake128State v_K) =
+    Core.Iter.Traits.Iterator.f_fold (Core.Iter.Traits.Collect.f_into_iter ({
+              Core.Ops.Range.f_start = sz 0;
+              Core.Ops.Range.f_end = v_K
+            }
+            <:
+            Core.Ops.Range.t_Range usize)
+        <:
+        Core.Ops.Range.t_Range usize)
+      (out, xof_state <: (t_Array (t_Array u8 (sz 504)) v_K & t_Shake128State v_K))
+      (fun temp_0_ i ->
+          let out, xof_state:(t_Array (t_Array u8 (sz 504)) v_K & t_Shake128State v_K) = temp_0_ in
+          let i:usize = i in
+          let tmp0, out1:(Libcrux.Hacl.Sha3.Incremental.t_Shake128State & t_Array u8 (sz 504)) =
+            Libcrux.Hacl.Sha3.Incremental.impl__Shake128State__squeeze_nblocks (sz 504)
+              (xof_state.f_state.[ i ] <: Libcrux.Hacl.Sha3.Incremental.t_Shake128State)
+          in
+          let xof_state:t_Shake128State v_K =
+            {
+              xof_state with
+              f_state
+              =
+              Rust_primitives.Hax.Monomorphized_update_at.update_at_usize xof_state.f_state i tmp0
+            }
+            <:
+            t_Shake128State v_K
+          in
+          let hoist3:t_Array u8 (sz 504) = out1 in
+          let hoist4:t_Array (t_Array u8 (sz 504)) v_K =
+            Rust_primitives.Hax.Monomorphized_update_at.update_at_usize out i hoist3
+          in
+          hoist4, xof_state <: (t_Array (t_Array u8 (sz 504)) v_K & t_Shake128State v_K))
+  in
+  let hax_temp_output:t_Array (t_Array u8 (sz 504)) v_K = out in
+  xof_state, hax_temp_output <: (t_Shake128State v_K & t_Array (t_Array u8 (sz 504)) v_K)
