proofs/fstar/extraction/Libcrux.Kem.Kyber.Hash_functions.fsti
@@ -3,6 +3,8 @@ module Libcrux.Kem.Kyber.Hash_functions
 open Core
 open FStar.Mul
 
+let v_BLOCK_SIZE: usize = sz 168
+
 val v_G (input: t_Slice u8) : Prims.Pure (t_Array u8 (sz 64)) Prims.l_True (fun _ -> Prims.l_True)
 
 val v_H (input: t_Slice u8) : Prims.Pure (t_Array u8 (sz 32)) Prims.l_True (fun _ -> Prims.l_True)
@@ -10,18 +12,27 @@ val v_H (input: t_Slice u8) : Prims.Pure (t_Array u8 (sz 32)) Prims.l_True (fun 
 val v_PRF (v_LEN: usize) (input: t_Slice u8)
     : Prims.Pure (t_Array u8 v_LEN) Prims.l_True (fun _ -> Prims.l_True)
 
-val v_XOF_absorb (v_K: usize) (input: t_Array (t_Array u8 (sz 34)) v_K)
-    : Prims.Pure (t_Array Libcrux.Digest.t_Shake128State v_K) Prims.l_True (fun _ -> Prims.l_True)
+let v_THREE_BLOCKS: usize = v_BLOCK_SIZE *! sz 3
 
-val v_XOF_free (v_K: usize) (xof_state: t_Array Libcrux.Digest.t_Shake128State v_K)
-    : Prims.Pure Prims.unit Prims.l_True (fun _ -> Prims.l_True)
+type t_Shake128State (v_K: usize) = {
+  f_state:t_Array Libcrux.Hacl.Sha3.Incremental.t_Shake128State v_K
+}
 
-val v_XOF_squeeze_block (v_K: usize) (xof_state: t_Array Libcrux.Digest.t_Shake128State v_K)
-    : Prims.Pure (t_Array (t_Array u8 (sz 168)) v_K & t_Array Libcrux.Digest.t_Shake128State v_K)
+val impl__new: v_K: usize -> Prims.unit
+  -> Prims.Pure (t_Shake128State v_K) Prims.l_True (fun _ -> Prims.l_True)
+
+val absorb (v_K: usize) (input: t_Array (t_Array u8 (sz 34)) v_K)
+    : Prims.Pure (t_Shake128State v_K) Prims.l_True (fun _ -> Prims.l_True)
+
+val free (v_K: usize) (xof_state: t_Shake128State v_K)
+    : Prims.Pure (t_Shake128State v_K) Prims.l_True (fun _ -> Prims.l_True)
+
+val squeeze_block (v_K: usize) (xof_state: t_Shake128State v_K)
+    : Prims.Pure (t_Shake128State v_K & t_Array (t_Array u8 (sz 168)) v_K)
       Prims.l_True
       (fun _ -> Prims.l_True)
 
-val v_XOF_squeeze_three_blocks (v_K: usize) (xof_state: t_Array Libcrux.Digest.t_Shake128State v_K)
-    : Prims.Pure (t_Array (t_Array u8 (sz 504)) v_K & t_Array Libcrux.Digest.t_Shake128State v_K)
+val squeeze_three_blocks (v_K: usize) (xof_state: t_Shake128State v_K)
+    : Prims.Pure (t_Shake128State v_K & t_Array (t_Array u8 (sz 504)) v_K)
       Prims.l_True
       (fun _ -> Prims.l_True)
